thys/Transition_Systems_and_Automata/Automata/DCA_Combine.thy
@@ -1,0 +1,139 @@
+section {* Deterministic Co-Büchi Automata Combinations *}
+
+theory DCA_Combine
+imports "DCA" "DGCA"
+begin
+
+  definition dcai :: "('label, 'state) dca list \<Rightarrow> ('label, 'state list) dca" where
+    "dcai AA \<equiv> dca
+      (INTER (set AA) dca.alphabet)
+      (map dca.initial AA)
+      (\<lambda> a pp. map2 (\<lambda> A p. dca.succ A a p) AA pp)
+      (\<lambda> pp. \<exists> k < length AA. dca.rejecting (AA ! k) (pp ! k))"
+
+  lemma dcai_trace_smap:
+    assumes "length pp = length AA" "k < length AA"
+    shows "smap (\<lambda> pp. pp ! k) (dca.trace (dcai AA) w pp) = dca.trace (AA ! k) w (pp ! k)"
+    using assms unfolding dcai_def by (coinduction arbitrary: w pp) (force)
+
+  lemma dcai_language: "DCA.language (dcai AA) = INTER (set AA) DCA.language"
+  proof safe
+    fix A w
+    assume 1: "w \<in> DCA.language (dcai AA)" "A \<in> set AA"
+    obtain 2:
+      "dca.run (dcai AA) w (dca.initial (dcai AA))"
+      "\<not> infs (dca.rejecting (dcai AA)) (dca.trace (dcai AA) w (dca.initial (dcai AA)))"
+      using 1(1) by rule
+    obtain k where 3: "A = AA ! k" "k < length AA" using 1(2) unfolding in_set_conv_nth by auto
+    have 4: "\<not> infs (\<lambda> pp. dca.rejecting A (pp ! k)) (dca.trace (dcai AA) w (map dca.initial AA))"
+      using 2(2) 3 unfolding dcai_def by auto
+    show "w \<in> DCA.language A"
+    proof
+      show "dca.run A w (dca.initial A)"
+        using 1(2) 2(1) unfolding DCA.run_alt_def dcai_def by auto
+      have "True \<longleftrightarrow> \<not> infs (\<lambda> pp. dca.rejecting A (pp ! k)) (dca.trace (dcai AA) w (map dca.initial AA))"
+        using 4 by simp
+      also have "\<dots> \<longleftrightarrow> \<not> infs (dca.rejecting A) (smap (\<lambda> pp. pp ! k)
+        (dca.trace (dcai AA) w (map dca.initial AA)))" by (simp add: comp_def)
+      also have "smap (\<lambda> pp. pp ! k) (dca.trace (dcai AA) w (map dca.initial AA)) =
+        dca.trace (AA ! k) w (map dca.initial AA ! k)" using 3(2) by (fastforce intro: dcai_trace_smap)
+      also have "\<dots> = dca.trace A w (dca.initial A)" using 3 by auto
+      finally show "\<not> infs (dca.rejecting A) (DCA.trace A w (dca.initial A))" by simp
+    qed
+  next
+    fix w
+    assume 1: "w \<in> INTER (set AA) DCA.language"
+    have 2: "dca.run A w (dca.initial A)" "\<not> infs (dca.rejecting A) (dca.trace A w (dca.initial A))"
+      if "A \<in> set AA" for A using 1 that by auto
+    have 3: "\<not> infs (\<lambda> pp. dca.rejecting (AA ! k) (pp ! k)) (dca.trace (dcai AA) w (map dca.initial AA))"
+      if "k < length AA" for k
+    proof -
+      have "True \<longleftrightarrow> \<not> infs (dca.rejecting (AA ! k)) (dca.trace (AA ! k) w (map dca.initial AA ! k))"
+        using 2(2) that by auto
+      also have "dca.trace (AA ! k) w (map dca.initial AA ! k) =
+        smap (\<lambda> pp. pp ! k) (dca.trace (dcai AA) w (map dca.initial AA))"
+        using that by (fastforce intro: dcai_trace_smap[symmetric])
+      also have "infs (dca.rejecting (AA ! k)) \<dots> \<longleftrightarrow> infs (\<lambda> pp. dca.rejecting (AA ! k) (pp ! k))
+        (dca.trace (dcai AA) w (map dca.initial AA))" by (simp add: comp_def)
+      finally show ?thesis by simp
+    qed
+    show "w \<in> DCA.language (dcai AA)"
+    proof
+      show "dca.run (dcai AA) w (dca.initial (dcai AA))"
+        using 2(1) unfolding DCA.run_alt_def dcai_def by auto
+      show "\<not> infs (dca.rejecting (dcai AA)) (dca.trace (dcai AA) w (dca.initial (dcai AA)))"
+        using 3 unfolding dcai_def by auto
+    qed
+  qed
+
+  definition dcau' :: "('label, 'state) dca list \<Rightarrow> ('label, 'state list) dgca" where
+    "dcau' AA \<equiv> dgca
+      (UNION (set AA) dca.alphabet)
+      (map dca.initial AA)
+      (\<lambda> a pp. map2 (\<lambda> A p. dca.succ A a p) AA pp)
+      (map (\<lambda> k pp. dca.rejecting (AA ! k) (pp ! k)) [0 ..< length AA])"
+
+  lemma dcau'_trace_smap:
+    assumes "length pp = length AA" "k < length AA"
+    shows "smap (\<lambda> pp. pp ! k) (dgca.trace (dcau' AA) w pp) = dca.trace (AA ! k) w (pp ! k)"
+    using assms unfolding dcau'_def by (coinduction arbitrary: w pp) (force)
+
+  lemma dcau'_language:
+    assumes "INTER (set AA) dca.alphabet = UNION (set AA) dca.alphabet"
+    shows "DGCA.language (dcau' AA) = UNION (set AA) DCA.language"
+  proof safe
+    fix w
+    assume 1: "w \<in> DGCA.language (dcau' AA)"
+    obtain k where 2:
+      "dgca.run (dcau' AA) w (dgca.initial (dcau' AA))"
+      "k < length AA"
+      "\<not> infs (\<lambda> pp. dca.rejecting (AA ! k) (pp ! k)) (dgca.trace (dcau' AA) w (dgca.initial (dcau' AA)))"
+      using 1 unfolding dcau'_def by force
+    show "w \<in> UNION (set AA) DCA.language"
+    proof (intro UN_I DCA.language)
+      show "AA ! k \<in> set AA" using 2(2) by simp
+      show "dca.run (AA ! k) w (dca.initial (AA ! k))"
+        using assms 2(1, 2) unfolding DCA.run_alt_def DGCA.run_alt_def dcau'_def by force
+      have "True \<longleftrightarrow> \<not> infs (\<lambda> pp. dca.rejecting (AA ! k) (pp ! k))
+        (dgca.trace (dcau' AA) w (map dca.initial AA))" using 2(3) unfolding dcau'_def by auto
+      also have "\<dots> \<longleftrightarrow> \<not> infs (dca.rejecting (AA ! k))
+        (smap (\<lambda> pp. pp ! k) (dgca.trace (dcau' AA) w (map dca.initial AA)))" by (simp add: comp_def)
+      also have "smap (\<lambda> pp. pp ! k) (dgca.trace (dcau' AA) w (map dca.initial AA)) =
+        dca.trace (AA ! k) w (map dca.initial AA ! k)" using 2(2) by (fastforce intro: dcau'_trace_smap)
+      also have "\<dots> = dca.trace (AA ! k) w (dca.initial (AA ! k))" using 2(2) by auto
+      finally show "\<not> infs (dca.rejecting (AA ! k)) (dca.trace (AA ! k) w (dca.initial (AA ! k)))" by simp
+    qed
+  next
+    fix A w
+    assume 1: "A \<in> set AA" "w \<in> DCA.language A"
+    obtain 2: "dca.run A w (dca.initial A)" "\<not> infs (dca.rejecting A) (dca.trace A w (dca.initial A))"
+      using 1(2) by rule
+    obtain k where 3: "A = AA ! k" "k < length AA" using 1(1) unfolding in_set_conv_nth by auto
+    show "w \<in> DGCA.language (dcau' AA)"
+    proof (intro DGCA.language bexI cogen)
+      show "dgca.run (dcau' AA) w (dgca.initial (dcau' AA))"
+        using 1(1) 2(1) unfolding DCA.run_alt_def DGCA.run_alt_def dcau'_def by auto
+      have "True \<longleftrightarrow> \<not> infs (dca.rejecting (AA ! k)) (dca.trace (AA ! k) w (map dca.initial AA ! k))"
+        using 2(2) 3 by auto
+      also have "dca.trace (AA ! k) w (map dca.initial AA ! k) =
+        smap (\<lambda> pp. pp ! k) (dgca.trace (dcau' AA) w (map dca.initial AA))"
+        using 3(2) by (fastforce intro: dcau'_trace_smap[symmetric])
+      also have "\<not> infs (dca.rejecting (AA ! k)) \<dots> \<longleftrightarrow> \<not> infs (\<lambda> pp. dca.rejecting (AA ! k) (pp ! k))
+        (dgca.trace (dcau' AA) w (map dca.initial AA))" by (simp add: comp_def)
+      also have "map dca.initial AA = dgca.initial (dcau' AA)" unfolding dcau'_def by simp
+      finally show "\<not> infs (\<lambda> pp. dca.rejecting (AA ! k) (pp ! k)) (dgca.trace (dcau' AA) w (dgca.initial (dcau' AA)))"
+        by simp
+      show "(\<lambda> pp. dca.rejecting (AA ! k) (pp ! k)) \<in> set (dgca.rejecting (dcau' AA))"
+        unfolding dcau'_def using 3(2) by simp
+    qed
+  qed
+
+  definition dcau :: "('label, 'state) dca list \<Rightarrow> ('label, 'state list degen) dca" where
+    "dcau = degen \<circ> dcau'"
+
+  lemma dcau_language:
+    assumes "INTER (set AA) dca.alphabet = UNION (set AA) dca.alphabet"
+    shows "DCA.language (dcau AA) = UNION (set AA) DCA.language"
+    unfolding dcau_def using degen_language dcau'_language[OF assms] by auto
+
+end
