thys/Transition_Systems_and_Automata/Automata/DGCA.thy
@@ -1,0 +1,77 @@
+section {* Deterministic Co-Generalized Co-Büchi Automata *}
+
+theory DGCA
+imports
+  "DCA"
+  "../Transition_Systems/Transition_System_Degeneralization"
+begin
+
+  datatype ('label, 'state) dgca = dgca
+    (alphabet: "'label set")
+    (initial: "'state")
+    (succ: "'label \<Rightarrow> 'state \<Rightarrow> 'state")
+    (rejecting: "'state pred gen")
+
+  global_interpretation dgca: transition_system_initial_generalized
+    "succ A" "\<lambda> a p. a \<in> alphabet A" "\<lambda> p. p = initial A" "rejecting A"
+    for A
+    defines path = dgca.path and run = dgca.run and reachable = dgca.reachable and nodes = dgca.nodes and
+      enableds = dgca.enableds and paths = dgca.paths and runs = dgca.runs and
+      dexecute = dgca.dexecute and denabled = dgca.denabled and dinitial = dgca.dinitial and
+      drejecting = dgca.dcondition
+    by this
+
+  abbreviation target where "target \<equiv> dgca.target"
+  abbreviation states where "states \<equiv> dgca.states"
+  abbreviation trace where "trace \<equiv> dgca.trace"
+
+  abbreviation successors :: "('label, 'state) dgca \<Rightarrow> 'state \<Rightarrow> 'state set" where
+    "successors \<equiv> dgca.successors TYPE('label)"
+
+  lemma path_alt_def: "path A w p \<longleftrightarrow> set w \<subseteq> alphabet A"
+  unfolding lists_iff_set[symmetric]
+  proof
+    show "w \<in> lists (alphabet A)" if "path A w p" using that by (induct arbitrary: p) (auto)
+    show "path A w p" if "w \<in> lists (alphabet A)" using that by (induct arbitrary: p) (auto)
+  qed
+  lemma run_alt_def: "run A w p \<longleftrightarrow> sset w \<subseteq> alphabet A"
+  unfolding streams_iff_sset[symmetric]
+  proof
+    show "w \<in> streams (alphabet A)" if "run A w p"
+      using that by (coinduction arbitrary: w p) (force elim: dgca.run.cases)
+    show "run A w p" if "w \<in> streams (alphabet A)"
+      using that by (coinduction arbitrary: w p) (force elim: streams.cases)
+  qed
+
+  definition language :: "('label, 'state) dgca \<Rightarrow> 'label stream set" where
+    "language A \<equiv> {w. run A w (initial A) \<and> cogen fins (rejecting A) (trace A w (initial A))}"
+
+  lemma language[intro]:
+    assumes "run A w (initial A)" "cogen fins (rejecting A) (trace A w (initial A))"
+    shows "w \<in> language A"
+    using assms unfolding language_def by auto
+  lemma language_elim[elim]:
+    assumes "w \<in> language A"
+    obtains "run A w (initial A)" "cogen fins (rejecting A) (trace A w (initial A))"
+    using assms unfolding language_def by auto
+
+  lemma language_alphabet: "language A \<subseteq> streams (alphabet A)"
+    unfolding language_def run_alt_def using sset_streams by auto
+
+  definition degen :: "('label, 'state) dgca \<Rightarrow> ('label, 'state degen) dca" where
+    "degen A \<equiv> dca (alphabet A) (The (dinitial A)) (dexecute A) (drejecting A)"
+
+  lemma degen_language: "DCA.language (degen A) = DGCA.language A"
+  proof -
+    have 1: "dca.trace (degen A) = dgca.degen.trace A" unfolding degen_def by simp
+    have 2: "dca.run (degen A) = dgca.degen.run A"
+      unfolding degen_def DCA.run_def DGCA.run_def dgca.denabled_def by (simp add: cond_case_prod_eta)
+    have 3: "dca.initial (degen A) = (dgca.initial A, 0)" unfolding degen_def dgca.dinitial_def by auto
+    have 4: "dca.rejecting (degen A) = drejecting A" unfolding degen_def by simp
+    show ?thesis
+      unfolding DCA.language_def DGCA.language_def 1 2 3 4
+      unfolding dgca.degen_run dgca.degen_infs run_def cogen_def
+      by auto
+  qed
+
+end
