thys/Transition_Systems_and_Automata/Automata/DRA_Combine.thy
@@ -1,0 +1,154 @@
+section {* Deterministic Rabin Automata Combinations *}
+
+theory DRA_Combine
+imports "DBA" "DCA" "DRA"
+begin
+
+  definition from_dba :: "('label, 'state) dba \<Rightarrow> ('label, 'state) dra" where
+    "from_dba A \<equiv> dra (dba.alphabet A) (dba.initial A) (dba.succ A) [(dba.accepting A, bot)]"
+
+  lemma from_dba_language: "DRA.language (from_dba A) = DBA.language A"
+    unfolding DBA.language_def DRA.language_def from_dba_def DBA.run_def DRA.run_def by (auto 0 3)
+
+  definition from_dca :: "('label, 'state) dca \<Rightarrow> ('label, 'state) dra" where
+    "from_dca A \<equiv> dra (dca.alphabet A) (dca.initial A) (dca.succ A) [(top, dca.rejecting A)]"
+
+  lemma from_dca_language: "DRA.language (from_dca A) = DCA.language A"
+    unfolding DCA.language_def DRA.language_def from_dca_def DCA.run_def DRA.run_def by (auto 0 3)
+
+  definition dbcai :: "('label, 'state\<^sub>1) dba \<Rightarrow> ('label, 'state\<^sub>2) dca \<Rightarrow> ('label, 'state\<^sub>1 \<times> 'state\<^sub>2) dra" where
+    "dbcai A B \<equiv> dra
+      (dba.alphabet A \<inter> dca.alphabet B)
+      (dba.initial A, dca.initial B)
+      (\<lambda> a (p, q). (dba.succ A a p, dca.succ B a q))
+      [(dba.accepting A \<circ> fst, dca.rejecting B \<circ> snd)]"
+
+  lemma dbcai_fst[iff]: "infs (P \<circ> fst) (dra.trace (dbcai A B) w (p, q)) \<longleftrightarrow> infs P (dba.trace A w p)"
+  proof -
+    have "infs (P \<circ> fst) (dra.trace (dbcai A B) w (p, q)) \<longleftrightarrow>
+      infs P (smap fst (dra.trace (dbcai A B) w (p, q)))" by simp
+    also have "smap fst (dra.trace (dbcai A B) w (p, q)) = dba.trace A w p"
+      unfolding dbcai_def by (coinduction arbitrary: w p q) (auto)
+    finally show ?thesis by this
+  qed
+  lemma dbcai_snd[iff]: "infs (P \<circ> snd) (dra.trace (dbcai A B) w (p, q)) \<longleftrightarrow> infs P (dca.trace B w q)"
+  proof -
+    have "infs (P \<circ> snd) (dra.trace (dbcai A B) w (p, q)) \<longleftrightarrow>
+      infs P (smap snd (dra.trace (dbcai A B) w (p, q)))" by simp
+    also have "smap snd (dra.trace (dbcai A B) w (p, q)) = dca.trace B w q"
+      unfolding dbcai_def by (coinduction arbitrary: w p q) (auto)
+    finally show ?thesis by this
+  qed
+
+  lemma dbcai_language: "DRA.language (dbcai A B) = DBA.language A \<inter> DCA.language B"
+  proof -
+    have 0: "dra.alphabet (dbcai A B) = dba.alphabet A \<inter> dca.alphabet B" unfolding dbcai_def by simp
+    have 1: "dra.initial (dbcai A B) = (dba.initial A, dca.initial B)" unfolding dbcai_def by simp
+    have 2: "dra.accepting (dbcai A B) = [(dba.accepting A \<circ> fst, dca.rejecting B \<circ> snd)]"
+      unfolding dbcai_def by simp
+    have 3: "cogen rabin (dra.accepting (dbcai A B)) (DRA.trace (dbcai A B) w (p, q)) \<longleftrightarrow>
+      infs (dba.accepting A) (DBA.trace A w p) \<and> fins (rejecting B) (DCA.trace B w q)" for w p q
+      unfolding cogen_def rabin_def 2 by simp
+    show ?thesis
+      unfolding DRA.language_def DBA.language_def DCA.language_def
+      unfolding DRA.run_alt_def DBA.run_alt_def DCA.run_alt_def
+      unfolding 0 1 3 by auto
+  qed
+
+  abbreviation (input) "get k pp \<equiv> pp ! k"
+
+  definition drau :: "('label, 'state) dra list \<Rightarrow> ('label, 'state list) dra" where
+    "drau AA \<equiv> dra
+      (UNION (set AA) dra.alphabet)
+      (map dra.initial AA)
+      (\<lambda> a pp. map2 (\<lambda> A p. dra.succ A a p) AA pp)
+      (do { k \<leftarrow> [0 ..< length AA]; (f, g) \<leftarrow> dra.accepting (AA ! k); [(f \<circ> get k, g \<circ> get k)] })"
+
+  lemma drau_trace:
+    assumes "length pp = length AA" "k < length AA"
+    shows "infs (P \<circ> get k) (dra.trace (drau AA) w pp) \<longleftrightarrow>
+      infs P (dra.trace (AA ! k) w (pp ! k))"
+  proof -
+    have "infs (P \<circ> get k) (dra.trace (drau AA) w pp) \<longleftrightarrow>
+      infs P (smap (get k) (dra.trace (drau AA) w pp))" by simp
+    also have "smap (get k) (dra.trace (drau AA) w pp) = dra.trace (AA ! k) w (pp ! k)"
+      using assms unfolding drau_def by (coinduction arbitrary: w pp) (force)
+    finally show ?thesis by this
+  qed
+
+  lemma drau_language:
+    assumes "INTER (set AA) dra.alphabet = UNION (set AA) dra.alphabet"
+    shows "DRA.language (drau AA) = UNION (set AA) DRA.language"
+  proof safe
+    fix w
+    assume 1: "w \<in> DRA.language (drau AA)"
+    obtain 2:
+      "dra.run (drau AA) w (dra.initial (drau AA))"
+      "cogen rabin (dra.accepting (drau AA)) (dra.trace (drau AA) w (dra.initial (drau AA)))"
+      using 1 by rule
+    obtain I F where 3:
+      "(I, F) \<in> set (dra.accepting (drau AA))"
+      "infs I (dra.trace (drau AA) w (dra.initial (drau AA)))"
+      "fins F (dra.trace (drau AA) w (dra.initial (drau AA)))"
+      using 2(2) by blast
+    obtain k P Q where 4:
+      "k < length AA" "I = P \<circ> get k" "F = Q \<circ> get k" "(P, Q) \<in> set (dra.accepting (AA ! k))"
+      using 3(1) unfolding drau_def List.bind_def by (auto simp: comp_def)
+    show "w \<in> UNION (set AA) DRA.language"
+    proof (intro UN_I DRA.language cogen rabin)
+      show "AA ! k \<in> set AA" using 4(1) by auto
+      show "DRA.run (AA ! k) w (dra.initial (AA ! k))"
+        using assms 2(1) 4(1) unfolding DRA.run_alt_def drau_def by force
+      show "(P, Q) \<in> set (dra.accepting (AA ! k))" using 4(4) by this
+      show "(P, Q) = (P, Q)" by rule
+      have "True \<longleftrightarrow> infs (P \<circ> get k) (dra.trace (drau AA) w (map dra.initial AA))"
+        using 3(2) unfolding drau_def 4(2) by simp
+      also have "\<dots> \<longleftrightarrow> infs P (dra.trace (AA ! k) w (map dra.initial AA ! k))"
+        using 4(1) by (force intro!: drau_trace)
+      also have "map dra.initial AA ! k = dra.initial (AA ! k)" using 4(1) by simp
+      finally show "infs P (dra.trace (AA ! k) w (dra.initial (AA ! k)))" by simp
+      have "False \<longleftrightarrow> infs (Q \<circ> get k) (dra.trace (drau AA) w (map dra.initial AA))"
+        using 3(3) unfolding drau_def 4(3) by simp
+      also have "\<dots> \<longleftrightarrow> infs Q (dra.trace (AA ! k) w (map dra.initial AA ! k))"
+        using 4(1) by (force intro!: drau_trace)
+      also have "map dra.initial AA ! k = dra.initial (AA ! k)" using 4(1) by simp
+      finally show "fins Q (dra.trace (AA ! k) w (dra.initial (AA ! k)))" by simp
+    qed
+  next
+    fix A w
+    assume 1: "A \<in> set AA" "w \<in> DRA.language A"
+    obtain 2:
+      "dra.run A w (dra.initial A)"
+      "cogen rabin (dra.accepting A) (dra.trace A w (dra.initial A))"
+      using 1(2) by rule
+    obtain I F where 3:
+      "(I, F) \<in> set (dra.accepting A)"
+      "infs I (dra.trace A w (dra.initial A))"
+      "fins F (dra.trace A w (dra.initial A))"
+      using 2(2) by blast
+    obtain k where 4: "A = AA ! k" "k < length AA" using 1(1) unfolding in_set_conv_nth by auto
+    show "w \<in> DRA.language (drau AA)"
+    proof (intro DRA.language cogen rabin)
+      show "dra.run (drau AA) w (dra.initial (drau AA))"
+        using 1(1) 2(1) unfolding DRA.run_alt_def drau_def by auto
+      show "(I \<circ> get k, F \<circ> get k) \<in> set (dra.accepting (drau AA))"
+        unfolding drau_def List.bind_def using 3(1) 4 by (force simp: comp_def)
+      show "(I \<circ> get k, F \<circ> get k) = (I \<circ> get k, F \<circ> get k)" by rule
+      have "infs (I \<circ> get k) (dra.trace (drau AA) w (dra.initial (drau AA))) \<longleftrightarrow>
+        infs (I \<circ> get k) (dra.trace (drau AA) w (map dra.initial AA))"
+        unfolding drau_def by simp
+      also have "\<dots> \<longleftrightarrow> infs I (dra.trace (AA ! k) w (map dra.initial AA ! k))"
+        using 4(2) by (force intro!: drau_trace)
+      also have "\<dots> \<longleftrightarrow> True" using 3(2) 4 by simp
+      finally show "infs (I \<circ> get k) (dra.trace (drau AA) w (dra.initial (drau AA)))" by simp
+      have "infs (F \<circ> get k) (dra.trace (drau AA) w (dra.initial (drau AA))) \<longleftrightarrow>
+        infs (F \<circ> get k) (dra.trace (drau AA) w (map dra.initial AA))"
+        unfolding drau_def by simp
+      also have "\<dots> \<longleftrightarrow> infs F (dra.trace (AA ! k) w (map dra.initial AA ! k))"
+        using 4(2) by (force intro!: drau_trace)
+      also have "\<dots> \<longleftrightarrow> False" using 3(3) 4 by simp
+      finally show "fins (F \<circ> get k) (dra.trace (drau AA) w (dra.initial (drau AA)))" by simp
+    qed
+  qed
+
+end
